Factor makefile, port to VST 2.11
1. Factor Makefile into separate make targets
2. Get the core CertiGraph to build in VST 2.11, CompCert 3.11
3. Much progress on getting CertiGC to build in VST 2.11

This is a checkpoint commit; right now all the
outputs-of-clightgen files are still from CompCert 3.10,
so you'll need to "make clightgen" to update them all.
I hope to fix that in a near-future commit,
and get more things to build.

CertiGC/spatial_gcgraph.v
@@ -54,8 +54,8 @@ Definition space_tri (sp: space): (reptype space_type) :=
   let s := sp.(space_start) in (s, (offset_val (WORD_SIZE * sp.(used_space)) s,
                                     offset_val (WORD_SIZE * sp.(total_space)) s)).
 
-Definition heap_struct_rep (sh: share) (sp_reps: list (reptype space_type)) (h: val):
-  mpred := data_at sh heap_type sp_reps h.
+Definition heap_struct_rep (sh: share) (sp_reps: list (@reptype CompSpecs space_type)) (h: val):
+  mpred := @data_at CompSpecs sh heap_type sp_reps h.
 
 Definition before_gc_thread_info_rep (sh: share) (ti: thread_info) (t: val) :=
   let nursery := heap_head ti.(ti_heap) in
@@ -489,17 +489,17 @@ Program Definition weak_derives (P Q: mpred): mpred := (! (P >=> Q))%pred.
 Lemma derives_nonexpansive: forall P Q n,
     approx n (weak_derives P Q) = approx n (weak_derives (approx n P) (approx n Q)).
 Proof.
-  apply nonexpansive2_super_non_expansive; repeat intro.
-  - split; simpl; intros; eapply H2 in H5; eauto;
-      assert (a >= level y0)%nat by (apply necR_level in H1; lia);
-      destruct (H _ H6).
-    + eapply H7; eauto.
-    + eapply H8; eauto.
-  - split; simpl; intros; eapply H2; eauto;
-      assert (a >= level y0)%nat by (apply necR_level in H1; lia);
-      destruct (H _ H6).
-    + eapply H8; eauto.
-    + eapply H7; eauto.
+  apply nonexpansive2_super_non_expansive; intros.
+  - split; simpl; intros;
+      (assert (a >= level a''0)%nat; [ | eapply H; eauto]);
+       apply ext_level in H6, H2;
+       apply necR_level in H1, H5;
+       lia.
+  - split; simpl; intros;
+      (assert (a >= level a''0)%nat; [ | eapply H in H7 ; eauto]);
+       apply ext_level in H6, H2;
+       apply necR_level in H1, H5;
+       lia.
 Qed.
 
 Lemma derives_nonexpansive_l: forall P Q n,
@@ -507,11 +507,18 @@ Lemma derives_nonexpansive_l: forall P Q n,
 Proof.
   repeat intro.
   apply (nonexpansive_super_non_expansive (fun P => weak_derives P Q)); repeat intro.
-  split; simpl; intros; eapply H2; eauto;
-    assert (a >= level y0)%nat by (apply necR_level in H1; lia);
-    destruct (H _ H6).
-  - eapply H8; eauto.
-  - eapply H7; eauto.
+  split; simpl; intros;
+   eapply H3; try eassumption.
+-
+   eapply H; auto.
+   apply ext_level in H6, H2;
+   apply necR_level in H1, H5.
+   lia.
+-
+   eapply H in H7; auto.
+   apply ext_level in H6, H2;
+   apply necR_level in H1, H5.
+   lia.
 Qed.
 
 Lemma derives_nonexpansive_r: forall P Q n,
@@ -519,11 +526,18 @@ Lemma derives_nonexpansive_r: forall P Q n,
 Proof.
   repeat intro.
   apply (nonexpansive_super_non_expansive (fun Q => weak_derives P Q)); repeat intro.
-  split; simpl; intros; eapply H2 in H5; eauto;
-    assert (a >= level y0)%nat by (apply necR_level in H1; lia);
-    destruct (H _ H6).
-  - eapply H7; eauto.
-  - eapply H8; eauto.
+  split; simpl; intros;
+   eapply H3 in H7; try eassumption.
+-
+   eapply H; auto.
+   apply ext_level in H6, H2;
+   apply necR_level in H1, H5.
+   lia.
+-
+   eapply H in H7; auto.
+   apply ext_level in H6, H2;
+   apply necR_level in H1, H5.
+   lia.
 Qed.
 
 Lemma derives_weak: forall P Q, P |-- Q -> TT |-- weak_derives P Q.
@@ -1241,17 +1255,17 @@ Proof.
 Qed.
 
 Definition space_struct_rep (sh: share) (tinfo: thread_info) (gen: nat) :=
-  data_at sh space_type (space_tri (nth_space tinfo gen)) (space_address tinfo gen).
+  @data_at CompSpecs sh space_type (space_tri (nth_space tinfo gen)) (space_address tinfo gen).
 
 Lemma heap_struct_rep_eq: forall sh l p,
-    heap_struct_rep sh l p = data_at sh (tarray space_type 12) l p.
+    heap_struct_rep sh l p = @data_at CompSpecs sh (tarray space_type 12) l p.
 Proof.
   intros. unfold heap_struct_rep. apply pred_ext; rewrite data_at_isptr; Intros.
-  - unfold_data_at (data_at _ heap_type _ _).
+  - unfold_data_at (@data_at CompSpecs _ heap_type _ _).
     entailer!. clear H0. rewrite field_at_data_at.
     unfold field_address. rewrite if_true by assumption. simpl.
     entailer!.
-  - unfold_data_at (data_at _ heap_type _ _). entailer!. clear H0 H1.
+  - unfold_data_at (@data_at CompSpecs _ heap_type _ _). entailer!. clear H0 H1.
     rewrite field_at_data_at. unfold field_address. rewrite if_true.
     + simpl. rewrite isptr_offset_val_zero by assumption. entailer!.
     + unfold field_compatible in *. simpl in *. intuition.
@@ -1279,8 +1293,8 @@ Lemma heap_struct_rep_split_lt: forall sh l tinfo i1 i2,
     i1 < MAX_SPACES -> i2 < MAX_SPACES -> 0 <= i1 < i2 -> Zlength l = MAX_SPACES ->
     exists B,
       heap_struct_rep sh l (ti_heap_p tinfo) =
-      data_at sh space_type (Znth i1 l) (space_address tinfo (Z.to_nat i1)) *
-      data_at sh space_type (Znth i2 l) (space_address tinfo (Z.to_nat i2)) * B.
+      @data_at CompSpecs sh space_type (Znth i1 l) (space_address tinfo (Z.to_nat i1)) *
+      @data_at CompSpecs sh space_type (Znth i2 l) (space_address tinfo (Z.to_nat i2)) * B.
 Proof.
   intros.
   exists (@data_at CompSpecs sh
@@ -1538,7 +1552,7 @@ Lemma ti_token_rep_add: forall ti sp i (Hs: 0 <= i < MAX_SPACES),
     ti_token_rep ti |-- ti_token_rep (ti_add_new_space ti sp i Hs).
 Proof.
   intros. unfold ti_token_rep. simpl. cancel. remember (spaces (ti_heap ti)).
-  rewrite <- (sublist_all (Zlength l) l) at 1 by lia.
+  rewrite <- (sublist_same 0 (Zlength l) l) at 1 by lia.
   assert (Zlength l = MAX_SPACES) by (subst; rewrite spaces_size; reflexivity).
   rewrite upd_Znth_unfold. 2: now rewrite H1.
   rewrite <- (sublist_rejoin 0 i) by lia. rewrite !iter_sepcon_app_sepcon. cancel.
@@ -1582,7 +1596,7 @@ Lemma heap_rest_rep_add: forall tinfo sp i (Hs: 0 <= i < MAX_SPACES),
     heap_rest_rep (ti_heap (ti_add_new_space tinfo sp i Hs)).
 Proof.
   intros. unfold heap_rest_rep. simpl. remember (spaces (ti_heap tinfo)).
-  rewrite <- (sublist_all (Zlength l) l) at 1 by lia.
+  rewrite <- (sublist_same 0 (Zlength l) l) at 1 by lia.
   assert (Zlength l = MAX_SPACES) by (subst; rewrite spaces_size; reflexivity).
   rewrite upd_Znth_unfold. 2: now rewrite H0.
   rewrite <- (sublist_rejoin 0 i) by lia. rewrite !iter_sepcon_app_sepcon.
