graph/SpaceAdjMatGraph1.v
@@ -2,21 +2,22 @@ Require Import Coq.ZArith.BinInt.
 Require Import Coq.ZArith.Zcomplements.
 Require Import Coq.micromega.Lia.
 Require Import Coq.ZArith.Znat.
-
+(*
 Require Import compcert.lib.Integers.
 Require Import compcert.common.Values.
 Require Import compcert.export.Clightdefs.
-
-Require Import VST.veric.mpred.
-Require Import VST.zlist.sublist.
-Require Import VST.floyd.field_at.
-Require Import VST.floyd.coqlib3.
+*)
+Require Import VST.floyd.proofauto.
+(*
 Require Import VST.msl.iter_sepcon.
 Require Import VST.msl.seplog.
+*)
+
 
 Require Import CertiGraph.graph.graph_model.
 Require Import CertiGraph.lib.List_ext.
 Require Import CertiGraph.graph.MathAdjMatGraph.
+Import invariants.
 
 Section Spatial_AdjMat_Model_1.
   (* Model 1 is for a heap-allocated graph,
@@ -30,7 +31,9 @@ Section Spatial_AdjMat_Model_1.
   Context {CompSpecs : compspecs}.
   Context {V_EqDec : EquivDec.EqDec V eq}.
   Context {E_EqDec: EquivDec.EqDec E eq}.
-
+Existing Instance V_EqDec.
+Existing Instance E_EqDec.
+(* Local Instance Inhabitant_val : Inhabitant val := Vundef. *)
   (* Assumption:
      (v,0), (v,1) ... (v, size-1) are edges.
 
@@ -128,7 +131,7 @@ Section Spatial_AdjMat_Model_1.
     rewrite nat_inc_list_i.
     2: rewrite Z2Nat_id', Z.max_r; lia.
     repeat rewrite iter_sepcon_app.
-    simpl. rewrite sepcon_emp. rewrite H.
+    simpl. rewrite predicates_sl.sepcon_emp. rewrite H.
     reflexivity.
   Qed.
 
